src/FrameStack/Termination.v
@@ -1,784 +1,232 @@
-Require Export SubstSemantics.
+From CoreErlang.FrameStack Require Export SubstSemantics.
 
 Import ListNotations.
 
-(** This property holds true if a ⟨fs, e⟩ configuration terminates. So it reaches a point with an empty FrameStack *)
-Definition terminates_sem (fs : FrameStack) (e : ProgResult) : Prop :=
-  exists v, ⟨fs, e⟩ -->* v.
+(** This property holds true if a |fs, e| configuration terminates in k steps. *)
+Definition terminates_in_k_sem (fs : FrameStack) (e : Redex) (k : nat)
+  : Prop :=
+  exists (res : Redex), is_result res /\ ⟨fs, e⟩ -[k]-> ⟨[], res⟩.
 
-(** This property holds true if a ⟨fs, e⟩ configuration terminates in k steps. So it reaches a point with an empty FrameStack in k steps *)
-Definition terminates_in_k_sem (fs : FrameStack) (e : ProgResult) (k : nat) : Prop :=
-  (*
-  (exists v, ⟨fs, e⟩ -[k]-> ⟨ [], ValSeqRes v⟩)
-  \/
-  (exists exc, ⟨fs, e⟩ -[k]-> ⟨ [], ExcRes exc⟩).
-  *)
-  (exists r, ⟨fs, e⟩ -[k]-> ⟨ [], r⟩ /\ ((exists v, r = ValSeqRes v) \/ (exists exc, r = ExcRes exc)))
-  .
-
-(* TODO: is this needed? *)
-(*Open Scope nat_scope. *)
 
 (** A more practical way to define termination in k steps *)
 Reserved Notation "| fs , e | k ↓" (at level 80).
-Inductive terminates_in_k : FrameStack -> ProgResult -> nat -> Prop :=
+Inductive terminates_in_k : FrameStack -> Redex -> nat -> Prop :=
 
 (** Ends *)
-| term_fin_val vs :
-  | [] , ValSeqRes vs | 0 ↓
-| term_fin_exc exc :
-  | [] , ExcRes exc | 0 ↓
+| term_fin v :
+  is_result v -> | [] , v | 0 ↓ 
 
+(** Cooling: single value *)
+| cool_value v xs k :
+  | xs, RValSeq [v] | k ↓
+->
+  | xs, `v | S k ↓
 
-(** Value ExpRess**)
+(************************************************)
+(* heating should be separate for all complex expressions (to be
+   syntax-driven).
+   Only the intermediate and last steps can be extracted: *)
+| step_params xs ident (el : list Exp) (vl : list Val) (v : Val) (e : Exp) k:
+  | FParams ident (vl ++ [v]) el :: xs, e | k ↓
+->
+  | FParams ident vl (e :: el) :: xs, RValSeq [v] | S k ↓
+
+(* technical rule to avoid duplication for 0 subexpressions : *)
+| step_params_0 xs ident e (el : list Exp) vl k:
+  |FParams ident vl el :: xs, RExp e| k ↓
+->
+  |FParams ident vl (e::el) ::xs, RBox| S k ↓
+
+(* 0 subexpression in complex expressions: *)
+| cool_params_0 xs ident (vl : list Val) (res : Redex) k: 
+  res = create_result ident vl ->
+  |xs, res| k ↓
+->
+  |FParams ident vl [] ::xs, RBox| S k ↓
+
+| cool_params xs ident (vl : list Val) (v : Val) (res : Redex) k:
+  res = create_result ident (vl ++ [v]) ->
+  |xs, res| k ↓
+->
+  |FParams ident vl [] :: xs, RValSeq [v]| S k ↓
+
+(************************************************)
+(* Heating constructs with list subexpressions: *)
+| heat_values (el : list Exp) (xs : list Frame) k:
+  | (FParams IValues [] el)::xs, RBox | k ↓
+->
+  | xs, EValues el | S k ↓
+
+| heat_tuple (el : list Exp) (xs : list Frame) k:
+  | (FParams ITuple [] el)::xs, RBox | k ↓ 
+->
+  | xs, ETuple el | S k ↓
+
+| heat_map (el : list (Exp * Exp)) (xs : list Frame) k:
+  | (FParams IMap [] (flatten_list el))::xs, RBox | k ↓ 
+->
+  | xs, EMap el | S k ↓
+
+| heat_call (el : list Exp) (xs : list Frame) f k:
+  | (FParams (ICall f) [] el)::xs, RBox | k ↓ 
+->
+  | xs, ECall f el | S k ↓
+
+| heat_primop (el : list Exp) (xs : list Frame) f k:
+  | (FParams (IPrimOp f) [] el)::xs, RBox | k ↓ 
+->
+  | xs, EPrimOp f el | S k ↓
+
+| heat_app2 (el : list Exp) (xs : list Frame) (v : Val) k:
+  | (FParams (IApp v) [] el)::xs, RBox | k ↓ 
+->
+  | FApp1 el :: xs, RValSeq [v] | S k ↓
+
+(************************************************)
+(**  App *)
+| heat_app xs e l k:
+  |FApp1 l :: xs, RExp e|  k ↓ 
+->
+  |xs, EApp e l| S k ↓
+(**  List *)
 (**  Cooling *)
-| term_cool_value v k fs:
-  | fs , ValSeqRes [v] | k ↓
-  ->
-  | fs , ExpRes (Val v) | (S k) ↓
 
+| cool_cons_1 (hd : Exp) (tl : Val) xs k :
+  | (FCons2 tl)::xs, RExp hd | k ↓ 
+->
+  | (FCons1 hd)::xs, RValSeq [tl] | S k ↓
 
-(**  Values *)
-(**  Cooling *)
-| term_cool_Values_empty k fs :
-  | fs , ValSeqRes [] | k ↓
-  ->
-  | fs , ExpRes (Exp (EValues [])) | (S k) ↓
-
-| term_cool_Values_1 vl e el v k fs :
-  | (FValues (vl++[v]) el)::fs , ExpRes e | k ↓
-  ->
-  | (FValues vl (e::el))::fs , ValSeqRes [v] | (S k) ↓
-
-| term_cool_Values_2 vl v k fs :
-  | fs , ValSeqRes (vl++[v]) | k ↓
-  ->
-  | (FValues vl [])::fs , ValSeqRes [v] | (S k) ↓
+| cool_cons_2 (hd tl : Val) xs k:
+  | xs, RValSeq [VCons hd tl] | k ↓ 
+->
+  | (FCons2 tl)::xs, RValSeq [hd] | S k ↓
 
 (**  Heating *)
-| term_heat_Values e el k fs:
-  | (FValues [] el)::fs , ExpRes e | k ↓
-  ->
-  | fs , ExpRes (Exp (EValues (e::el))) | (S k) ↓
-
-
-(**  Cons *)
-(**  Cooling *)
-| term_cool_Cons_1 hd tl k fs :
-  | (FCons2 tl)::fs , ExpRes hd | k ↓
-  ->
-  | (FCons1 hd)::fs , ValSeqRes [tl] | (S k) ↓
-
-| term_cool_Cons_2 hd tl k fs :
-  | fs ,ValSeqRes [VCons hd tl] | k ↓
-  ->
-  | (FCons2 tl)::fs , ValSeqRes [hd] | (S k) ↓
-
-(**  Heating *)
-| term_heat_Cons hd tl k fs :
-  | (FCons1 hd)::fs , ExpRes tl | k ↓
-  ->
-  | fs , ExpRes (Exp (ECons hd tl)) | (S k) ↓
-
-
-(**  Tuple *)
-(**  Cooling *)
-| term_cool_Tuple_empty k fs :
-  | fs , ValSeqRes [ VTuple [] ] | k ↓
-  ->
-  | fs , ExpRes (Exp (ETuple [])) | (S k) ↓
-
-| term_cool_Tuple_1 vl e el v k fs :
-  | (FTuple (vl++[v]) el)::fs , ExpRes e | k ↓
-  ->
-  | (FTuple vl (e::el))::fs , ValSeqRes [v] | (S k) ↓
-
-| term_cool_Tuple_2 vl v k fs :
-  | fs , ValSeqRes [ VTuple (vl++[v]) ] | k ↓
-  ->
-  | (FTuple vl [])::fs , ValSeqRes [v] | (S k) ↓
-
-(**  Heating *)
-| term_heat_Tuple e el k xs:
-  | (FTuple [] el)::xs , ExpRes e | k ↓
-  ->
-  | xs , ExpRes (Exp (ETuple (e::el))) | (S k) ↓
-
-
-(**  Map *)
-(**  Cooling *)
-| term_cool_Map_empty k fs :
-    | fs , ValSeqRes [ VMap [] ] | k ↓
-  ->
-  | fs , ExpRes (Exp (EMap [])) | (S k) ↓
-
-| term_cool_Map_1  vl sn fs el k xs :
-  | (FMap2 vl fs el)::xs , ExpRes sn | k ↓
-  ->
-  | (FMap1 vl sn el)::xs , ValSeqRes [fs] | (S k) ↓
-
-| term_cool_Map_2  vl fs sn fs' sn' el k xs :
-  | (FMap1 (vl++[(fs,sn)]) sn' el)::xs , ExpRes fs' | k ↓
-  ->
-  | (FMap2 vl fs ((fs',sn')::el))::xs , ValSeqRes [sn] | (S k) ↓
-
-| term_cool_Map_3  vl fs sn k xs :
-  | xs , ValSeqRes [ VMap (vl++[(fs,sn)]) ] | k ↓
-  ->
-  | (FMap2 vl fs [])::xs , ValSeqRes [sn] | (S k) ↓
-
-(**  Heating *)
-| term_heat_Map fs sn el k xs :
-  | (FMap1 [] sn el)::xs , ExpRes fs | k ↓
-  ->
-  | xs , ExpRes (Exp (EMap ((fs,sn)::el))) | (S k) ↓
-
-
-(**  PrimOp *) (* "inl res" is a ValueExpRes*)
-(**  Cooling *)
-| term_cool_PrimOp_empty f k xs res eff :
-  eval f [] [] = (inl res, eff) ->
-  | xs , ValSeqRes res | k ↓
-  ->
-  | xs , ExpRes(Exp (EPrimOp f [])) | (S k) ↓
-
-| term_cool_PrimOp_1 f vl e el v k xs :
-  | (FPrimOp f (vl++[v]) el)::xs , ExpRes e | k ↓
-  ->
-  | (FPrimOp f vl (e::el))::xs , ValSeqRes [v] | (S k) ↓
-
-| term_cool_PrimOp_2 f vl v k xs res eff :
-  eval f (vl++[v]) [] = (inl res, eff) ->
-  | xs , ValSeqRes res | k ↓
-  ->
-  | (FPrimOp f vl [])::xs , ValSeqRes [v] | (S k) ↓
-
-(**  Heating *)
-| term_heat_PrimOp f e el k xs :
-  | (FPrimOp f [] el)::xs , ExpRes e | k ↓
-  ->
-  | xs , ExpRes (Exp (EPrimOp f (e::el))) | (S k) ↓
-
-(** Exceptions *)
-| term_err_PrimOp_1 f k xs exc eff : (* in this case there were no parameters to evaluate *)
-  eval f [] [] = (inr exc, eff) ->
-  | xs , ExcRes exc | k ↓
-  ->
-  | xs , ExpRes (Exp (EPrimOp f [])) | (S k) ↓
-
-| term_err_PrimOp_2 f vl v k xs exc eff : (* there were parameters *)
-  eval f (vl++[v]) [] = (inr exc, eff) ->
-  | xs , ExcRes exc | k ↓
-  ->
-  | (FPrimOp f vl [])::xs , ValSeqRes [v] | (S k) ↓
-
+| heat_cons (hd tl : Exp) xs k:
+  | (FCons1 hd)::xs, RExp tl | k ↓ 
+->
+  | xs, ECons hd tl | S k ↓
 
 (**  Let *)
 (**  Cooling *)
-| term_cool_Let l e2 vs k xs :
+| cool_let l e2 vs xs k:
   length vs = l ->
-  | xs , ExpRes (e2.[ list_subst vs idsubst ]) | k ↓
-  ->
-  | (FLet l e2)::xs , ValSeqRes vs | (S k) ↓
-(**  Heating *)
-| term_heat_Let l e1 e2 k xs :
-  | (FLet l e2)::xs , ExpRes e1 | k ↓
-  ->
-  | xs , ExpRes (Exp (ELet l e1 e2)) | (S k) ↓
+  | xs, RExp (e2.[ list_subst vs idsubst ]) | k ↓ 
+->
+  | (FLet l e2)::xs, RValSeq vs | S k ↓
 
+(**  Heating *)
+| heat_let l e1 e2 xs k:
+  | (FLet l e2)::xs, RExp e1 | k ↓ 
+->
+  | xs, ELet l e1 e2 | S k ↓
 
 (**  Seq *)
 (**  Cooling *)
-| term_cool_Seq e2 v k xs :
-  | xs , ExpRes e2 | k ↓
-  ->
-  | (FSeq e2)::xs , ValSeqRes [v] | (S k) ↓
+| cool_seq e2 v xs k:
+  | xs, RExp e2 | k ↓ 
+->
+  | (FSeq e2)::xs, RValSeq [v] | S k ↓
 (**  Heating *)
-| term_heat_Seq e1 e2 k xs :
-  | (FSeq e2)::xs , ExpRes e1 | k ↓
-  ->
-  | xs , ExpRes (Exp (ESeq e1 e2)) | (S k) ↓
+| heat_seq e1 e2 xs k:
+  | (FSeq e2)::xs, RExp e1 | k ↓ 
+->
+  | xs, ESeq e1 e2 | S k ↓
 
 
 (**  Fun *)
 (**  Cooling *)
-| term_cool_fun e vl k xs :
-  | xs , ValSeqRes [ VClos [] 0 vl e ] | k ↓        (*TODO : id not 0*)
-  ->
-  | xs , ExpRes (Exp (EFun vl e)) | (S k) ↓
-
-
-(**  Call *)
-(**  Cooling *)
-| term_cool_Call_empty f k xs res eff :
-  eval f [] [] = (inl res, eff) ->
-  | xs , ValSeqRes res | k ↓
-  ->
-  | xs , ExpRes (Exp (ECall f [])) | (S k) ↓
-
-| term_cool_Call_1 f vl e el v k xs :
-  | (FCall f (vl++[v]) el)::xs , ExpRes e | k ↓
-  ->
-  | (FCall f vl (e::el))::xs , ValSeqRes [v] | (S k) ↓
-
-| term_cool_Call_2 f vl v k xs res eff :
-  eval f (vl++[v]) [] = (inl res, eff) ->
-  | xs , ValSeqRes res | k ↓
-  ->
-  | (FCall f vl [])::xs , ValSeqRes [v] | (S k) ↓
-
-(**  Heating *)
-| term_heat_Call f e el k xs :
-  | (FCall f [] el)::xs , ExpRes e | k ↓
-  ->
-  | xs , ExpRes (Exp (ECall f (e::el))) | (S k) ↓
-
-(** Exceptions *)
-| term_err_Call_1 f exc eff k xs : (* in this case there were no parameters to evaluate *)
-  eval f [] [] = (inr exc, eff) ->
-  | xs , ExcRes exc | k ↓
-  ->
-  | xs , ExpRes (Exp (ECall f [])) | (S k) ↓
-
-| term_err_Call_2 f v vl exc eff k xs : (* there were parameters *)
-  eval f (vl++[v]) [] = (inr exc, eff) ->
-  | xs , ExcRes exc | k ↓
-  ->
-  | (FCall f vl [])::xs , ValSeqRes [v] | (S k) ↓
-
-
-(**  App *) (* in "EApp e el" e needs to evaluate to a VClos but it will only be checked when el is done *)
-(**  Cooling *)
-| term_cool_App_empty vl' ext id e k xs :
-  convert_to_closlist ext = vl' ->
-  | xs , ExpRes e.[list_subst (vl') idsubst] | k ↓
-  ->
-  | (FApp1 [])::xs , ValSeqRes [(VClos ext id 0 e)] | (S k) ↓
-
-| term_cool_App_1 e el v k xs :
-  | (FApp2 v [] el)::xs , ExpRes e | k ↓
-  ->
-  | (FApp1 (e::el))::xs , ValSeqRes [v] | (S k) ↓
-
-| term_cool_App_2a v' vl e el v k xs :
-  | (FApp2 v' (vl++[v]) el)::xs , ExpRes e | k ↓
-  ->
-  | (FApp2 v' vl (e::el))::xs , ValSeqRes [v] | (S k) ↓
-
-| term_cool_App_2b vl' ext id vc e' vl v k xs :
-  vc = (length (vl) + 1) ->
-  convert_to_closlist ext = vl' ->
-  | xs , ExpRes (e'.[list_subst (vl'++(vl++[v])) idsubst]) | k ↓
-  ->
-  | (FApp2 (VClos ext id vc e') vl [])::xs , ValSeqRes [v] | (S k) ↓
-
-(**  Heating *)
-| term_heat_App e el k xs :
-  | (FApp1 el)::xs , ExpRes e | k ↓
-  ->
-  | xs , ExpRes (Exp (EApp e el)) | (S k) ↓
-
-(** Exceptions *) (*TODO badarity FApp1 version*)
-| term_err_App_badariry_1 ext id vc e k xs :
-  vc <> 0 ->
-  | xs , ExcRes (badarity (VClos ext id vc e)) | k ↓
-  ->
-  | (FApp1 [])::xs , ValSeqRes [(VClos ext id vc e)] | (S k) ↓
-
-| term_err_App_badariry_2 ext id vc e' vl k xs v :
-  vc <> (length (vl) + 1) ->
-  | xs , ExcRes (badarity (VClos ext id vc e')) | k ↓
-  ->
-  | (FApp2 (VClos ext id vc e') vl [])::xs , ValSeqRes [v] | (S k) ↓
-
-| term_err_App_noclos_1 v k xs : (* when it had no other expressions to evalate ([] case) *)
-  (forall ext id vc e, v <> (VClos ext id vc e)) ->
-  | xs , ExcRes (badfun v) | k ↓
-  ->
-  | (FApp1 [])::xs , ValSeqRes [v] | (S k) ↓
-
-| term_err_App_noclos_2 v' vl v k xs : (* when it had expressions to evaluate *)
-  (forall ext id vc e', v' <> (VClos ext id vc e')) ->
-  | xs , ExcRes (badfun v') | k ↓
-  ->
-  | (FApp2 v' vl [])::xs , ValSeqRes [v] | (S k) ↓
+| cool_fun e vl xs k:
+  | xs, RValSeq [ VClos [] 0 vl e ] | k ↓ 
+->
+  | xs, EFun vl e | S k ↓
+  (* TODO : id <> 0 usually *)
 
 
 (**  Case *)
-(**  Cooling *)
-| term_cool_Case_1m lp e1 e2 l vs vs' k xs :
-  match_pattern_list lp vs = Some vs' ->
-  | (FCase2 vs lp e2 l vs')::xs , ExpRes (e1.[list_subst (vs') idsubst]) | k ↓
-  ->
-  | (FCase1 ((lp,e1,e2)::l))::xs , ValSeqRes vs | (S k) ↓
-
-| term_cool_Case_1nm lp e1 e2 l vs k xs :
-  match_pattern_list lp vs = None ->
-  | (FCase1 l)::xs , ValSeqRes vs | k ↓
-  ->
-  | (FCase1 ((lp,e1,e2)::l))::xs , ValSeqRes vs | (S k) ↓
-
-| term_cool_Case_2mt vs lp e' l vs' k xs :
-  | xs , ExpRes (e'.[list_subst (vs') idsubst]) | k ↓
-  ->
-  | (FCase2 vs lp e' l vs')::xs , ValSeqRes [ VLit (Atom "true") ] | (S k) ↓
-
-| term_cool_Case_2mf vs lp' e' l vs' k xs :
-  | (FCase1 l)::xs , ValSeqRes vs | k ↓
-  ->
-  | (FCase2 vs lp' e' l vs')::xs , ValSeqRes [ VLit (Atom "false") ] | (S k) ↓
-
 (**  Heating *)
-| term_heat_Case e l k xs:
-  | (FCase1 l)::xs , ExpRes e | k ↓
-  ->
-  | xs , ExpRes (Exp (ECase e l)) | (S k) ↓
+| heat_Case e l xs k:
+  | (FCase1 l)::xs, RExp e | k ↓ 
+->
+  | xs, ECase e l | S k ↓
+
+(**  Cooling *)
+(* reduction started or it is already ongoing, the first pattern matched,
+   e1 the guard needs to be evaluated. vs' (the result of the pattern
+   matching is stored in the frame) *)
+| step_case_match lp e1 e2 l vs vs' xs k:
+  match_pattern_list lp vs = Some vs' ->
+  | (FCase2 vs lp e2 l vs')::xs, RExp (e1.[list_subst vs' idsubst]) | k ↓
+->
+  | (FCase1 ((lp,e1,e2)::l))::xs, RValSeq vs | S k ↓
+(* reduction started or it is already ongoing, the first pattern doesn't 
+   match, so we check the next pattern *)
+| step_case_not_match lp e1 e2 l vs xs k:
+  match_pattern_list lp vs = None ->
+  | (FCase1 l)::xs, RValSeq vs | k ↓ 
+->
+  | (FCase1 ((lp,e1,e2)::l))::xs, RValSeq vs | S k ↓
+
+(* reduction is ongoing, the pattern matched, and the guard is true, thus 
+   the reduction continues inside the given clause *)
+| step_case_true vs lp e' l vs' xs k:
+  | xs, RExp (e'.[list_subst vs' idsubst]) | k ↓ 
+->
+  | (FCase2 vs lp e' l vs')::xs, RValSeq [ VLit (Atom "true") ] | S k ↓
+
+(* reduction is ongoing, the pattern matched, and the guard is false, thus
+   we check the next pattern. *)
+| step_case_false vs lp' e' l vs' xs k:
+  | (FCase1 l)::xs, RValSeq vs | k ↓ 
+->
+  | (FCase2 vs lp' e' l vs')::xs, RValSeq [ VLit (Atom "false") ] | S k ↓
 
 (** Exceptions *)
-| term_err_Case_empty vs k xs:
-  | xs , ExcRes if_clause | k ↓
-  ->
-  | (FCase1 [])::xs , ValSeqRes vs | (S k) ↓
-
+| cool_case_empty vs xs k:
+  | xs, RExc if_clause | k ↓ 
+->
+  | (FCase1 [])::xs, RValSeq vs | S k ↓
 
 (**  LetRec *)
+(**  Cooling *)
 (**  Heating *)
-| term_heat_LetRec l e lc k xs :
-  convert_to_closlist (map (fun '(x,y) => (0,x,y)) l) = lc -> (*TODO: for now the funids are 0 coded in *)
-  | xs , ExpRes e.[list_subst (lc) idsubst] | k ↓
-  ->
-  | xs , ExpRes (Exp (ELetRec l e)) | (S k) ↓
+| heat_LetRec l e lc xs k:
+  convert_to_closlist (map (fun '(x,y) => (0,x,y)) l) = lc ->
+  (* TODO: for now the funids are 0 coded in *)
+  | xs, RExp e.[list_subst lc idsubst] | k ↓ 
+->
+  | xs, ELetRec l e | S k ↓
 
 
 (**  Try *)
 (**  Cooling *)
-| term_cool_Try_ok vl1 e2 vl2 e3 vs k xs:
+| cool_Try_ok vl1 e2 vl2 e3 vs xs k:
   vl1 = length vs ->
-  | xs , ExpRes e2.[ list_subst vs idsubst ] | k ↓
-  ->
-  | (FTry vl1 e2 vl2 e3)::xs , ValSeqRes vs | (S k) ↓
-
-| term_cool_Try_err vl1 e2 e3 class reason details k xs:  (* in CErlang exceptions always have 3 part*)
-  | xs , ExpRes e3.[ list_subst [exclass_to_value class; reason; details] idsubst ] | k ↓
-  ->
-  | (FTry vl1 e2 3 e3)::xs , ExcRes (class, reason, details) | (S k) ↓
-
+  | xs, RExp e2.[ list_subst vs idsubst ] | k ↓ 
+->
+  | (FTry vl1 e2 vl2 e3)::xs, RValSeq vs | S k ↓
+| cool_Try_err vl1 e2 e3 class reason details xs k:
+  (* in Core Erlang exceptions always have 3 parts *)
+  | xs, RExp e3.[ list_subst [exclass_to_value class; reason; details] idsubst ] | k ↓
+->
+  | (FTry vl1 e2 3 e3)::xs, RExc (class, reason, details) | S k ↓
 (**  Heating *)
-| term_heat_Try e1 vl1 e2 vl2 e3 k xs :
-  | (FTry vl1 e2 vl2 e3)::xs , ExpRes e1 | k ↓
-  ->
-  | xs , ExpRes (Exp (ETry e1 vl1 e2 vl2 e3)) | (S k) ↓
-
-
+| heat_Try e1 vl1 e2 vl2 e3 xs k:
+  | (FTry vl1 e2 vl2 e3)::xs, RExp e1 | k ↓ 
+->
+  | xs, ETry e1 vl1 e2 vl2 e3 | S k ↓
+  
 (** Exceptions *)
 (** Propogation *)
-| term_propogate_Exception frame exc k xs :
-  (forall vl1 e2 vl2 e3 , (FTry vl1 e2 vl2 e3) <> frame)->
-  | xs , ExcRes exc | k ↓
-  ->
-  | (frame)::xs , ExcRes exc | (S k) ↓
-
+| propogate_Exception F exc xs k:
+  (forall vl1 e2 vl2 e3, (FTry vl1 e2 vl2 e3) <> F) ->
+  | xs, RExc exc | k ↓ 
+->
+  | F::xs, RExc exc | S k ↓
+  (* TODO: details could be appended here to the stack trace *)
 where "| fs , e | k ↓" := (terminates_in_k fs e k).
 
-(** A more practical way to define termination *)
-Definition terminates (fs : FrameStack) (e : ProgResult) := exists n, | fs, e | n ↓.
+Definition terminates (fs : FrameStack) (e : Redex) :=
+  exists n, | fs, e | n ↓.
 Notation "| fs , e | ↓" := (terminates fs e) (at level 80).
-
-
-Theorem terminates_in_k_eq_terminates_in_k_sem :
-  forall k e fs, terminates_in_k_sem fs e k <-> | fs, e | k ↓.
-Proof.
-  
-  intros. split; revert e fs.
-  * induction k.
-    - intros. destruct H. destruct H. inversion H. subst. destruct H0.
-      + destruct H0. subst. constructor.
-      + destruct H0. subst. constructor.
-    - intros. destruct H. destruct H. inversion H. subst. specialize (IHk e' fs').
-      (* pose proof (conj H5 H0). Check ex_intro. apply ex_intro with (x := x) in H1. *)
-      assert (terminates_in_k_sem fs' e' k).
-      {
-        unfold terminates_in_k_sem. exists x. split; auto.
-      }
-      specialize (IHk H1). clear H H0 H5 H1. inversion H2; subst.
-      + constructor. auto.
-      + constructor. auto.
-      + constructor. auto.
-      + constructor. auto.
-      + constructor. auto.
-      + constructor. auto.
-      + constructor. auto.
-      + constructor. auto.
-      + constructor. auto.
-      + constructor. auto.
-      + constructor. auto.
-      + constructor. auto.
-      + constructor. auto.
-      + constructor. auto.
-      + constructor. auto.
-      + constructor. auto.
-      + constructor. auto.
-      + eapply term_cool_PrimOp_empty.
-        ** exact H.
-        ** auto.
-      + constructor. auto.
-      + econstructor.
-        ** exact H.
-        ** auto.
-      + constructor. auto.
-      + eapply term_err_PrimOp_1.
-        ** exact H.
-        ** auto.
-      + eapply term_err_PrimOp_2.
-        ** exact H.
-        ** auto.
-      + constructor.
-        ** auto.
-        ** auto.
-      + constructor. auto.
-      + constructor. auto.
-      + constructor. auto.
-      + constructor. auto.
-      + eapply term_cool_Call_empty.
-        ** exact H.
-        ** auto.
-      + eapply term_cool_Call_1. auto.
-      + eapply term_cool_Call_2.
-        ** exact H.
-        ** auto.
-      + constructor. auto.
-      + eapply term_err_Call_1.
-        ** exact H.
-        ** auto.
-      + eapply term_err_Call_2.
-        ** exact H.
-        ** auto.
-      + Check term_cool_App_empty. apply (term_cool_App_empty (convert_to_closlist ext)).
-        ** auto.
-        ** auto.
-      + constructor. auto.
-      + constructor. auto.
-      + Check term_cool_App_2b. apply (term_cool_App_2b (convert_to_closlist ext)).
-        ** auto.
-        ** auto.
-        ** auto.
-      + constructor. auto.
-      + apply (term_err_App_badariry_1).
-        ** auto.
-        ** auto.
-      + apply term_err_App_badariry_2.
-        ** auto.
-        ** auto.
-      + apply term_err_App_noclos_1.
-        ** auto.
-        ** auto.
-      + apply term_err_App_noclos_2.
-        ** auto.
-        ** auto.
-      + eapply term_cool_Case_1m.
-        ** exact H.
-        ** auto.
-      + apply term_cool_Case_1nm.
-        ** auto.
-        ** auto.
-      + constructor. auto.
-      + constructor. auto.
-      + constructor. auto.
-      + constructor. auto.
-      + Check term_heat_LetRec. eapply (term_heat_LetRec _ _ (convert_to_closlist (map (fun '(x0, y) => (0, x0, y)) l))).
-        ** auto.
-        ** auto.
-      + eapply term_cool_Try_ok.
-        ** auto.
-        ** auto.
-      + constructor. auto.
-      + constructor. auto.
-      + eapply term_propogate_Exception.
-        ** auto.
-        ** auto.
-  * intros. induction H.
-    - unfold terminates_in_k_sem. exists (ValSeqRes vs). split.
-      + constructor.
-      + left. exists vs. auto.
-    - unfold terminates_in_k_sem. exists (ExcRes exc). split.
-      + constructor.
-      + right. exists exc. auto.
-    - unfold terminates_in_k_sem. destruct IHterminates_in_k. destruct H0. exists x.
-      split.
-      + econstructor.
-        ** constructor.
-        ** auto.
-      + auto.
-    - unfold terminates_in_k_sem. destruct IHterminates_in_k. destruct H0. exists x. split.
-      + econstructor.
-        ** constructor.
-        ** auto.
-      + auto.
-    - unfold terminates_in_k_sem. destruct IHterminates_in_k. destruct H0. exists x. split.
-      + econstructor.
-        ** constructor.
-        ** auto.
-      + auto.
-    - unfold terminates_in_k_sem. destruct IHterminates_in_k. destruct H0. exists x. split.
-      + econstructor.
-        ** constructor.
-        ** auto.
-      + auto.
-    - unfold terminates_in_k_sem. destruct IHterminates_in_k. destruct H0. exists x. split.
-      + econstructor.
-        ** constructor.
-        ** auto.
-      + auto.
-    - unfold terminates_in_k_sem. destruct IHterminates_in_k. destruct H0. exists x. split.
-      + econstructor.
-        ** constructor.
-        ** auto.
-      + auto.
-    - unfold terminates_in_k_sem. destruct IHterminates_in_k. destruct H0. exists x. split.
-      + econstructor.
-        ** constructor.
-        ** auto.
-      + auto.
-    - unfold terminates_in_k_sem. destruct IHterminates_in_k. destruct H0. exists x. split.
-      + econstructor.
-        ** constructor.
-        ** auto.
-      + auto.
-    - unfold terminates_in_k_sem. destruct IHterminates_in_k. destruct H0. exists x. split.
-      + econstructor.
-        ** constructor.
-        ** auto.
-      + auto.
-    - unfold terminates_in_k_sem. destruct IHterminates_in_k. destruct H0. exists x. split.
-      + econstructor.
-        ** constructor.
-        ** auto.
-      + auto.
-    - unfold terminates_in_k_sem. destruct IHterminates_in_k. destruct H0. exists x. split.
-      + econstructor.
-        ** constructor.
-        ** auto.
-      + auto.
-    - unfold terminates_in_k_sem. destruct IHterminates_in_k. destruct H0. exists x. split.
-      + econstructor.
-        ** constructor.
-        ** auto.
-      + auto.
-    - unfold terminates_in_k_sem. destruct IHterminates_in_k. destruct H0. exists x. split.
-      + econstructor.
-        ** constructor.
-        ** auto.
-      + auto.
-    - unfold terminates_in_k_sem. destruct IHterminates_in_k. destruct H0. exists x. split.
-      + econstructor.
-        ** constructor.
-        ** auto.
-      + auto.
-    - unfold terminates_in_k_sem. destruct IHterminates_in_k. destruct H0. exists x. split.
-      + econstructor.
-        ** constructor.
-        ** auto.
-      + auto.
-    - unfold terminates_in_k_sem. destruct IHterminates_in_k. destruct H0. exists x. split.
-      + econstructor.
-        ** constructor.
-        ** auto.
-      + auto.
-    - unfold terminates_in_k_sem. destruct IHterminates_in_k. destruct H0. exists x. split.
-      + econstructor.
-        ** constructor.
-        ** auto.
-      + auto.
-    - unfold terminates_in_k_sem. destruct IHterminates_in_k. destruct H1. exists x. split.
-      + econstructor.
-        ** econstructor. exact H.
-        ** auto.
-      + auto.
-    - unfold terminates_in_k_sem. destruct IHterminates_in_k. destruct H0. exists x. split.
-      + econstructor.
-        ** constructor.
-        ** auto.
-      + auto.
-    - unfold terminates_in_k_sem. destruct IHterminates_in_k. destruct H1. exists x. split.
-      + econstructor.
-        ** econstructor. exact H.
-        ** auto.
-      + auto.
-    - unfold terminates_in_k_sem. destruct IHterminates_in_k. destruct H0. exists x. split.
-      + econstructor.
-        ** constructor.
-        ** auto.
-      + auto.
-    - unfold terminates_in_k_sem. destruct IHterminates_in_k. destruct H1. exists x. split.
-      + econstructor.
-        ** eapply err_PrimOp_1. exact H.
-        ** auto.
-      + auto.
-    - unfold terminates_in_k_sem. destruct IHterminates_in_k. destruct H1. exists x. split.
-      + econstructor.
-        ** eapply err_PrimOp_2. exact H.
-        ** auto.
-      + auto.
-    - unfold terminates_in_k_sem. destruct IHterminates_in_k. destruct H1. exists x. split.
-      + econstructor.
-        ** constructor. auto.
-        ** auto.
-      + auto.
-    - unfold terminates_in_k_sem. destruct IHterminates_in_k. destruct H0. exists x. split.
-      + econstructor.
-        ** constructor.
-        ** auto.
-      + auto.
-    - unfold terminates_in_k_sem. destruct IHterminates_in_k. destruct H0. exists x. split.
-      + econstructor.
-        ** constructor.
-        ** auto.
-      + auto.
-    - unfold terminates_in_k_sem. destruct IHterminates_in_k. destruct H0. exists x. split.
-      + econstructor.
-        ** constructor.
-        ** auto.
-      + auto.
-    - unfold terminates_in_k_sem. destruct IHterminates_in_k. destruct H0. exists x. split.
-      + econstructor.
-        ** constructor.
-        ** auto.
-      + auto.
-    - unfold terminates_in_k_sem. destruct IHterminates_in_k. destruct H1. exists x. split.
-      + econstructor.
-        ** eapply cool_Call_empty. exact H.
-        ** auto.
-      + auto.
-    - unfold terminates_in_k_sem. destruct IHterminates_in_k. destruct H0. exists x. split.
-      + econstructor.
-        ** constructor.
-        ** auto.
-      + auto.
-    - unfold terminates_in_k_sem. destruct IHterminates_in_k. destruct H1. exists x. split.
-      + econstructor.
-        ** eapply cool_Call_2. exact H.
-        ** auto.
-      + auto.
-    - unfold terminates_in_k_sem. destruct IHterminates_in_k. destruct H0. exists x. split.
-      + econstructor.
-        ** constructor.
-        ** auto.
-      + auto.
-    - unfold terminates_in_k_sem. destruct IHterminates_in_k. destruct H1. exists x. split.
-      + econstructor.
-        ** eapply err_Call_1. exact H.
-        ** auto.
-      + auto.
-    - unfold terminates_in_k_sem. destruct IHterminates_in_k. destruct H1. exists x. split.
-      + econstructor.
-        ** eapply err_Call_2. exact H.
-        ** auto.
-      + auto.
-    - unfold terminates_in_k_sem. destruct IHterminates_in_k. destruct H1. exists x. split.
-      + econstructor.
-        ** eapply cool_App_empty. exact H.
-        ** auto.
-      + auto.
-    - unfold terminates_in_k_sem. destruct IHterminates_in_k. destruct H0. exists x. split.
-      + econstructor.
-        ** constructor.
-        ** auto.
-      + auto.
-    - unfold terminates_in_k_sem. destruct IHterminates_in_k. destruct H0. exists x. split.
-      + econstructor.
-        ** constructor.
-        ** auto.
-      + auto.
-    - unfold terminates_in_k_sem. destruct IHterminates_in_k. destruct H2. exists x. split.
-      + econstructor.
-        ** constructor.
-           -- auto.
-           -- exact H0.
-        ** auto.
-      + auto.
-    - unfold terminates_in_k_sem. destruct IHterminates_in_k. destruct H0. exists x. split.
-      + econstructor.
-        ** constructor.
-        ** auto.
-      + auto.
-    - unfold terminates_in_k_sem. destruct IHterminates_in_k. destruct H1. exists x. split.
-      + econstructor.
-        ** constructor. auto.
-        ** auto.
-      + auto.
-    - unfold terminates_in_k_sem. destruct IHterminates_in_k. destruct H1. exists x. split.
-      + econstructor.
-        ** apply err_App_badariry_2. auto.
-        ** auto.
-      + auto.
-    - unfold terminates_in_k_sem. destruct IHterminates_in_k. destruct H1. exists x. split.
-      + econstructor.
-        ** constructor. auto.
-        ** auto.
-      + auto.
-    - unfold terminates_in_k_sem. destruct IHterminates_in_k. destruct H1. exists x. split.
-      + econstructor.
-        ** constructor. auto.
-        ** auto.
-      + auto.
-    - unfold terminates_in_k_sem. destruct IHterminates_in_k. destruct H1. exists x. split.
-      + econstructor.
-        ** apply cool_Case_1m. exact H.
-        ** auto.
-      + auto.
-    - unfold terminates_in_k_sem. destruct IHterminates_in_k. destruct H1. exists x. split.
-      + econstructor.
-        ** apply cool_Case_1nm. auto.
-        ** auto.
-      + auto.
-    - unfold terminates_in_k_sem. destruct IHterminates_in_k. destruct H0. exists x. split.
-      + econstructor.
-        ** constructor.
-        ** auto.
-      + auto.
-    - unfold terminates_in_k_sem. destruct IHterminates_in_k. destruct H0. exists x. split.
-      + econstructor.
-        ** constructor.
-        ** auto.
-      + auto.
-    - unfold terminates_in_k_sem. destruct IHterminates_in_k. destruct H0. exists x. split.
-      + econstructor.
-        ** constructor.
-        ** auto.
-      + auto.
-    - unfold terminates_in_k_sem. destruct IHterminates_in_k. destruct H0. exists x. split.
-      + econstructor.
-        ** constructor.
-        ** auto.
-      + auto.
-    - unfold terminates_in_k_sem. destruct IHterminates_in_k. destruct H1. exists x. split.
-      + econstructor.
-        ** constructor. exact H.
-        ** auto.
-      + auto.
-    - unfold terminates_in_k_sem. destruct IHterminates_in_k. destruct H1. exists x. split.
-      + econstructor.
-        ** constructor. auto.
-        ** auto.
-      + auto.
-    - unfold terminates_in_k_sem. destruct IHterminates_in_k. destruct H0. exists x. split.
-      + econstructor.
-        ** constructor.
-        ** auto.
-      + auto.
-    - unfold terminates_in_k_sem. destruct IHterminates_in_k. destruct H0. exists x. split.
-      + econstructor.
-        ** constructor.
-        ** auto.
-      + auto.
-    - unfold terminates_in_k_sem. destruct IHterminates_in_k. destruct H1. exists x. split.
-      + econstructor.
-        ** constructor. auto.
-        ** auto.
-      + auto.
-Qed.
-
-
-
-
 
