src/FrameStack/SubstSemanticsLemmas.v
@@ -1,7 +1,419 @@
-Require Export SubstSemantics.
+From CoreErlang.FrameStack Require Export SubstSemantics Termination.
 From Coq Require Export Logic.ProofIrrelevance Program.Equality.
-
 Import ListNotations.
+
+(* TODO: Is this needed? *)
+(* if there is two identical hypotheses then this tac will clear one *)
+Ltac proof_irr :=
+match goal with
+| [H1 : ?P, H2 : ?P |- _] => assert (H1 = H2) by apply proof_irrelevance; subst
+end.
+Ltac proof_irr_many := repeat proof_irr.
+
+(** Properties of the semantics *)
+Theorem step_determinism {e e' fs fs'} :
+  ⟨ fs, e ⟩ --> ⟨fs', e'⟩ ->
+  (forall fs'' e'', ⟨fs, e⟩ --> ⟨fs'', e''⟩ -> fs'' = fs' /\ e'' = e').
+Proof.
+  intro H. dependent induction H; intros;
+  match goal with
+  | [H : ⟨ _, _ ⟩ --> ⟨_, _⟩ |- _] => inversion H; subst; auto
+  end.
+  (* case: *)
+  * rewrite H in H9. inversion H9; now subst.
+  * rewrite H in H9; congruence.
+  * rewrite H in H9; congruence.
+  (* exceptions: *)
+  * specialize (H5 vl1 e2 3 e3). congruence.
+  * specialize (H vl1 e2 3 e3). congruence.
+Qed.
+
+Theorem value_nostep v :
+  is_result v ->
+  forall fs' v', ⟨ [], v ⟩ --> ⟨fs' , v'⟩ -> False.
+Proof.
+  intros H fs' v' HD. inversion H; subst; inversion HD.
+Qed.
+
+Theorem step_rt_determinism {e v fs fs' k} :
+  ⟨fs, e⟩ -[k]-> ⟨fs', v⟩
+->
+  (forall fs'' v', ⟨fs, e⟩ -[k]-> ⟨fs'', v'⟩ -> fs' = fs'' /\ v' = v).
+Proof.
+  intro. dependent induction H; intros.
+  * inversion H; subst; auto.
+  * inversion H1; subst. apply IHstep_rt; auto. eapply step_determinism in H; eauto. destruct H. subst. auto.
+Qed.
+
+Print Frame.
+Ltac destruct_scope :=
+  match goal with
+  | [H : RED _ ⊢ (RExp _) |- _] => inversion H; subst; clear H
+  | [H : RED _ ⊢ (RValSeq _) |- _] => inversion H; subst; clear H
+  | [H : RED _ ⊢ (RExc _) |- _] => inversion H; subst; clear H
+  | [H : RED _ ⊢ RBox |- _] => clear H
+  | [H : FSCLOSED (_ :: _) |- _] => inversion H; subst; clear H
+  | [H : FSCLOSED [] |- _] => clear H
+  | [H : EXP _ ⊢ VVal _ |- _] => inversion H; subst; clear H
+  | [H : EXP _ ⊢ EExp _ |- _] => inversion H; subst; clear H
+  | [H : VAL _ ⊢ VNil |- _] => clear H
+  | [H : VAL _ ⊢ VLit _ |- _] => clear H
+  | [H : VAL _ ⊢ VCons _ _ |- _] => inversion H; subst; clear H
+  | [H : VAL _ ⊢ VTuple _ |- _] => inversion H; subst; clear H
+  | [H : VAL _ ⊢ VMap _ |- _] => inversion H; subst; clear H
+  | [H : VAL _ ⊢ VVar _ |- _] => inversion H; subst; clear H
+  | [H : VAL _ ⊢ VFunId _ |- _] => inversion H; subst; clear H
+  | [H : VAL _ ⊢ VClos _ _ _ _ |- _] => inversion H; subst; clear H
+  | [H : NVAL _ ⊢ EFun _ _ |- _] => inversion H; subst; clear H
+  | [H : NVAL _ ⊢ EValues _ |- _] => inversion H; subst; clear H
+  | [H : NVAL _ ⊢ ECons _ _ |- _] => inversion H; subst; clear H
+  | [H : NVAL _ ⊢ ETuple _ |- _] => inversion H; subst; clear H
+  | [H : NVAL _ ⊢ EMap _ |- _] => inversion H; subst; clear H
+  | [H : NVAL _ ⊢ ECall _ _ |- _] => inversion H; subst; clear H
+  | [H : NVAL _ ⊢ EPrimOp _ _ |- _] => inversion H; subst; clear H
+  | [H : NVAL _ ⊢ EApp _ _ |- _] => inversion H; subst; clear H
+  | [H : NVAL _ ⊢ ECase _ _ |- _] => inversion H; subst; clear H
+  | [H : NVAL _ ⊢ ELet _ _ _ |- _] => inversion H; subst; clear H
+  | [H : NVAL _ ⊢ ESeq _ _ |- _] => inversion H; subst; clear H
+  | [H : NVAL _ ⊢ ELetRec _ _ |- _] => inversion H; subst; clear H
+  | [H : NVAL _ ⊢ ETry _ _ _ _ _ |- _] => inversion H; subst; clear H
+  | [H : FCLOSED (FCons1 _) |- _] => inversion H; subst; clear H
+  | [H : FCLOSED (FCons2 _) |- _] => inversion H; subst; clear H
+  | [H : FCLOSED (FParams _ _ _) |- _] => inversion H; subst; clear H
+  | [H : FCLOSED (FApp1 _) |- _] => inversion H; subst; clear H
+  | [H : FCLOSED (FCase1 _) |- _] => inversion H; subst; clear H
+  | [H : FCLOSED (FCase2 _ _ _ _ _) |- _] => inversion H; subst; clear H
+  | [H : FCLOSED (FLet _ _) |- _] => inversion H; subst; clear H
+  | [H : FCLOSED (FSeq _) |- _] => inversion H; subst; clear H
+  | [H : FCLOSED (FTry _ _ _ _) |- _] => inversion H; subst; clear H
+  end.
+
+Ltac destruct_scopes := repeat destruct_scope.
+
+Ltac destruct_forall :=
+  match goal with
+  | [H : Forall _ (_ :: _) |- _] => inversion H; subst; clear H
+  | [H : Forall _ [] |- _] => clear H
+  end.
+
+Ltac destruct_foralls := repeat destruct_forall.
+
+#[global]
+Hint Constructors RedexScope : core. 
+
+Lemma deflatten_keeps_prop {A} (P : A -> Prop) :
+  forall (l : list A),
+    Forall P l ->
+    Forall (fun '(x, y) => P x /\ P y) (deflatten_list l).
+Proof.
+  induction l using list_length_ind.
+  intro HF.
+  destruct l. 2: destruct l.
+  * constructor.
+  * cbn. constructor.
+  * cbn. inversion HF. inversion H3. subst.
+    clear HF H3. constructor; auto.
+    apply H; simpl; auto.
+Qed.
+
+Lemma map_insert_prop :
+  forall (P : Val * Val -> Prop) l k v,
+    P (k, v) ->
+    Forall P l ->
+    Forall P (map_insert k v l).
+Proof.
+  induction l; intros k v HP HF.
+  * constructor; auto.
+  * simpl. destruct a as [k' v'].
+    destruct_foralls.
+    break_match_goal. 2: break_match_goal.
+    - constructor. 2: constructor. all: auto.
+    - constructor; auto.
+    - constructor; auto.
+Qed.
+
+Lemma make_val_map_keeps_prop (P : Val * Val -> Prop) :
+  forall l,
+    Forall P l ->
+    Forall P (make_val_map l).
+Proof.
+  induction l; intro H.
+  * constructor.
+  * cbn. destruct a. inversion H. subst. clear H.
+    apply IHl in H3. clear IHl.
+    now apply map_insert_prop.
+Qed.
+
+Lemma flatten_keeps_prop {A} (P : A -> Prop) :
+  forall (l : list (A * A)),
+    Forall (fun '(x, y) => P x /\ P y) l ->
+    Forall P (flatten_list l).
+Proof.
+  induction l; intros; simpl in *; auto.
+  destruct a.
+  destruct_foralls. destruct H2. constructor; auto.
+Qed.
+
+Lemma closlist_scope Γ ext :
+  (forall i : nat,
+  i < Datatypes.length ext ->
+  EXP Datatypes.length ext + nth i (map (snd ∘ fst) ext) 0 + Γ
+  ⊢ nth i (map snd ext) (` VNil))
+  ->
+  Forall (fun v : Val => VAL Γ ⊢ v) (convert_to_closlist ext).
+Proof.
+  unfold convert_to_closlist. intros. induction ext.
+  * constructor.
+  * constructor.
+    - destruct a, p. specialize (H 0 ltac:(simpl;lia)) as H'.
+      simpl in H'. constructor.
+      + simpl. intros. apply H. simpl; auto.
+      + simpl. exact H'.
+    - assert (forall i : nat,
+                  i < Datatypes.length ext ->
+                  EXP Datatypes.length ext + nth i (map (snd ∘ fst) ext) 0 + Γ
+                  ⊢ nth i (map snd ext) (` VNil)). {
+        intros.
+      }
+Admitted. (* TODO: this should hold, but the induction is tricky! *)
+
+#[global]
+Hint Constructors ValScoped : core.
+#[global]
+Hint Constructors ExpScoped : core.
+#[global]
+Hint Constructors NonValScoped : core.
+#[global]
+Hint Constructors ICLOSED : core.
+ 
+
+Lemma subtract_elem_closed :
+  forall v1 v2, VALCLOSED v1 -> VALCLOSED v2 ->
+  VALCLOSED (subtract_elem v1 v2).
+Proof.
+  induction v1; intros; cbn; try constructor.
+  repeat break_match_goal; destruct_scopes; auto.
+Qed.
+
+Theorem closed_eval : forall m f vl eff,
+  Forall (fun v => VALCLOSED v) vl ->
+  REDCLOSED (fst (eval m f vl eff)).
+Proof.
+  intros. unfold eval.
+  break_match_goal; unfold eval_arith, eval_logical, eval_equality,
+  eval_transform_list, eval_list_tuple, eval_cmp, eval_io,
+  eval_hd_tl, eval_elem_tuple, eval_check, eval_error; try rewrite Heqb.
+  all: try destruct vl; try destruct vl.
+  all: simpl; try (now (constructor; constructor)).
+  all: repeat break_match_goal.
+  all: try (constructor; constructor); auto.
+  all: try now constructor; auto.
+  all: destruct_foralls; destruct_scopes; auto.
+  all: try (apply indexed_to_forall; repeat constructor; auto).
+  * constructor. apply indexed_to_forall. repeat constructor. auto.
+  * clear Heqb eff m f. induction v; cbn.
+    all: try (do 2 constructor; apply indexed_to_forall; do 2 constructor; now auto).
+    - now do 2 constructor.
+    - destruct_scopes. apply IHv1 in H4 as H4'. break_match_goal.
+      2: break_match_goal. 3: break_match_goal.
+      all: try (do 2 constructor; apply indexed_to_forall; now repeat constructor).
+      do 3 constructor; subst; auto.
+      apply IHv2 in H5. destruct_scopes. now destruct_foralls.
+  * clear Heqb eff m f. generalize dependent v. induction v0; intros; cbn; break_match_goal; try destruct v.
+    all: try (do 2 constructor; apply indexed_to_forall; do 2 constructor; now auto).
+    1-3: destruct_scopes; do 3 constructor; auto.
+    destruct_scopes. destruct v0_2; cbn in *.
+    3: {
+      apply IHv0_2; auto.
+      repeat break_match_goal; auto.
+      constructor; auto.
+      now apply subtract_elem_closed.
+    }
+    all: repeat break_match_goal; auto.
+    all: constructor; constructor; auto.
+    all: try apply subtract_elem_closed; auto.
+    all: constructor; auto; now apply subtract_elem_closed.
+  * clear Heqb eff m f. induction v; cbn.
+    all: destruct_scopes; try (do 2 constructor; apply indexed_to_forall; now repeat constructor).
+    do 2 constructor; auto. induction l; constructor.
+    - apply (H1 0). simpl. lia.
+    - apply IHl. intros. apply (H1 (S i)). simpl. lia.
+  * clear Heqb eff m f. generalize dependent v. induction l; cbn; intros.
+    - constructor. simpl. lia.
+    - destruct v; cbn in Heqs; try congruence.
+      destruct_scopes. 
+      repeat break_match_hyp; inversion Heqs; subst.
+      constructor. apply indexed_to_forall. constructor; auto.
+      apply IHl in Heqs0; auto.
+      constructor. apply indexed_to_forall. constructor; auto.
+      inversion Heqs0. now rewrite <- indexed_to_forall in H1.
+  * clear Heqb eff m f. generalize dependent e. induction v; cbn; intros.
+    all: try congruence.
+    all: try inversion Heqs; subst; clear Heqs.
+    all: try (do 2 constructor; apply indexed_to_forall; do 2 constructor; now auto).
+    destruct (transform_list v2) eqn:Eq.
+    - destruct v2; try congruence; inversion H0; subst.
+      all: try (do 2 constructor; apply indexed_to_forall; do 2 constructor; now auto).
+    - destruct v2; try congruence; inversion H0; subst.
+      all: try (do 2 constructor; apply indexed_to_forall; do 2 constructor; now auto).
+      apply IHv2; auto. destruct_scopes. auto.
+  * epose proof (proj1 (nth_error_Some l0 (Init.Nat.pred (Pos.to_nat p))) _).
+    Unshelve. 2: { intro. rewrite H in Heqo. congruence. }
+    eapply nth_error_nth with (d := VNil) in Heqo. subst. now apply H2.
+  * remember (Init.Nat.pred (Pos.to_nat p)) as k. clear Heqk Heqb m f p eff.
+    generalize dependent l2. revert k. induction l0; intros; simpl in *.
+    - destruct k; congruence.
+    - destruct k.
+      + inversion Heqo. subst. constructor.
+        intros. destruct i; simpl in *.
+        auto.
+        apply (H2 (S i)). lia.
+      + break_match_hyp. 2: congruence.
+        inversion Heqo; subst; clear Heqo. constructor. simpl.
+        intros. destruct i.
+        apply (H2 0). lia.
+        apply IHl0 in Heqo0. inversion Heqo0. apply (H4 i). lia.
+        intros. apply (H2 (S i0)). lia.
+  * apply indexed_to_forall in H1. destruct_foralls. now constructor.
+  * apply indexed_to_forall in H1. destruct_foralls. now constructor. 
+Qed.
+
+
+
+
+Theorem create_result_closed :
+  forall vl ident,
+    Forall (fun v => VALCLOSED v) vl ->
+    ICLOSED ident ->
+    REDCLOSED (create_result ident vl).
+Proof.
+  intros vl ident Hall Hi.
+  destruct ident; simpl.
+  1-3: constructor; auto.
+  1-2: do 2 constructor; auto.
+  * now apply (indexed_to_forall _ (fun v => VALCLOSED v) VNil).
+  * apply deflatten_keeps_prop in Hall.
+    apply make_val_map_keeps_prop in Hall.
+    rewrite indexed_to_forall in Hall. Unshelve. 2: exact (VNil, VNil).
+    intros. specialize (Hall i H).
+    replace VNil with (fst (VNil, VNil)) by auto. rewrite map_nth.
+    destruct nth. apply Hall.
+  * apply deflatten_keeps_prop in Hall.
+    apply make_val_map_keeps_prop in Hall.
+    rewrite indexed_to_forall in Hall. Unshelve. 2: exact (VNil, VNil).
+    intros. specialize (Hall i H).
+    replace VNil with (snd (VNil, VNil)) by auto. rewrite map_nth.
+    destruct nth. apply Hall.
+  * now apply closed_eval.
+  * now apply closed_eval.
+  * inversion Hi; subst; clear Hi. destruct v; unfold badfun.
+    1-7: constructor; auto; constructor.
+    break_match_goal.
+    - constructor. destruct_scope.
+      apply -> subst_preserves_scope_exp. exact H6.
+      apply Nat.eqb_eq in Heqb. rewrite Heqb.
+      replace (Datatypes.length ext + Datatypes.length vl + 0) with
+              (length (convert_to_closlist ext ++ vl)).
+      2: { unfold convert_to_closlist.
+           rewrite app_length, map_length. lia.
+      }
+      apply scoped_list_idsubst. apply Forall_app; split; auto.
+      now apply closlist_scope.
+    - unfold badarity. constructor. constructor. auto.
+Qed.
+
+Lemma Forall_pair {A B} (P1 : A -> Prop) (P2 : B -> Prop) l : forall d1 d2,
+  (forall i : nat,
+  i < Datatypes.length l -> P1 (nth i (map fst l) d1)) ->
+  (forall i : nat,
+    i < Datatypes.length l -> P2 (nth i (map snd l) d2)) ->
+  Forall (fun '(x, y) => P1 x /\ P2 y) l.
+Proof.
+  induction l; intros; constructor.
+  * destruct a. split. apply (H 0). simpl. lia. apply (H0 0). simpl. lia.
+  * eapply IHl; intros.
+    apply (H (S i)). simpl. lia.
+    apply (H0 (S i)). simpl. lia.
+Qed.
+
+Theorem step_closedness : forall F e F' e',
+   ⟨ F, e ⟩ --> ⟨ F', e' ⟩ -> FSCLOSED F -> REDCLOSED e
+->
+  FSCLOSED F' /\ REDCLOSED e'.
+Proof.
+  intros F e F' e' IH. induction IH; intros Hcl1 Hcl2;
+  destruct_scopes; destruct_foralls; split; auto.
+  all: cbn; try (repeat constructor; now auto).
+  all: try now (apply indexed_to_forall in H1; do 2 (constructor; auto)).
+  * constructor; auto. constructor; auto.
+    apply Forall_app; auto.
+  * now apply create_result_closed.
+  * apply create_result_closed; auto. apply Forall_app; auto.
+  * do 2 (constructor; auto).
+    epose proof (Forall_pair _ _ _ _ _ H0 H3).
+    now apply flatten_keeps_prop.
+  * do 2 (constructor; auto).
+    now apply indexed_to_forall in H4.
+  * constructor. apply -> subst_preserves_scope_exp.
+    eassumption.
+    now apply scoped_list_idsubst.
+  * constructor; auto. constructor.
+    now rewrite Nat.add_0_r in H5.
+  * admit.
+  * admit.
+  * admit.
+  * admit.
+  * admit.
+  * constructor. apply -> subst_preserves_scope_exp.
+    eassumption.
+    apply scoped_list_idsubst.  
+Qed.
+
+Theorem result_VALCLOSED_any (fs : FrameStack) (e v : Exp) :
+  ⟨ fs, e ⟩ -->* v -> VALCLOSED v.
+Proof.
+  intros. destruct H. auto.
+Qed.
+
+Corollary step_any_closedness : forall F e v,
+   ⟨ F, e ⟩ -->* v -> FSCLOSED F -> EXPCLOSED e
+->
+  VALCLOSED v.
+Proof.
+  intros. destruct H, H2. induction H2.
+  * destruct e; try inversion H; now inversion H1.
+  * apply step_closedness in H2; auto.
+Qed.
+
+
+
+
+
+Theorem terminates_in_k_eq_terminates_in_k_sem :
+  forall k e fs, terminates_in_k_sem fs e k <-> | fs, e | k ↓.
+Proof.
+  split.
+  {
+    revert e fs. induction k; intros e fs H.
+    * destruct H as [res [Hres HD]].
+      inversion HD; subst. now constructor.
+    * destruct H as [res [Hres HD]].
+      inversion HD; subst.
+      assert (terminates_in_k_sem fs' e' k). {
+        eexists. split; eassumption.
+      }
+      apply IHk in H.
+  }
+Qed.
+
+
+
+
+
+
+
+
+
 
 (** This theorem says that the semantics rules are deterministic. *)
 Theorem semmantics_rules_determinism :
@@ -48,14 +460,6 @@ intros. inversion H; subst; inversion H0; auto; subst.
 * specialize (H6 vl1 e0 3 e3). congruence.
 * specialize (H1 vl1 e0 3 e3). congruence.
 Qed.
-
-(* TODO: Is this needed? *)
-(* if there is two identical hip then this tac will clear one *)
-Ltac proof_irr :=
-match goal with
-| [H1 : ?P, H2 : ?P |- _] => assert (H1 = H2) by apply proof_irrelevance; subst
-end.
-Ltac proof_irr_many := repeat proof_irr.
 
 
 Theorem step_rt_determinism :
